checkpoint

pulse/lib/pulse/lib/Pulse.Lib.Barrier.fst
@@ -20,7 +20,9 @@ noeq type barrier_t = {
   core: barrier_t_core;
   i: iref
 }
+
 let full_perm : perm = 1.0R
+
 let empty_map_below (n:nat)
 : carrier
 = Map.map_literal 
@@ -91,6 +93,57 @@ let recv (b:barrier_t) (q:storable)
     barrier b p **
     big_ghost_pcm_pts_to b.core.gref (singleton i #0.5R q)
 
+```pulse
+ghost
+fn unfold_map_invariant0 v m n p
+requires map_invariant v m n p ** pure (v == 0ul)
+ensures pure (p == OR.on_range (predicate_at m) 0 n /\ all_perms m 0 n 0.5R)
+{
+  rewrite each v as 0ul;
+  unfold map_invariant;
+  unfold map_invariant0;
+}
+```
+
+```pulse
+ghost
+fn fold_map_invariant0 m n (p:storable)
+requires pure (p == OR.on_range (predicate_at m) 0 n /\ all_perms m 0 n 0.5R)
+ensures map_invariant 0ul m n p
+{
+  fold (map_invariant0 m n p);
+  fold (map_invariant 0ul m n p)
+}
+```
+
+```pulse
+ghost
+fn fold_map_invariant1 v m n p
+requires
+  OR.on_range (predicate_at m) 0 n **
+  pure (all_perms m 0 n 0.5R) **
+  pure (v =!= 0ul)
+ensures
+  map_invariant v m n p
+{
+  rewrite (OR.on_range (predicate_at m) 0 n ** pure (all_perms m 0 n 0.5R))
+  as      map_invariant v m n p
+}
+```
+
+```pulse
+ghost
+fn unfold_map_invariant1 v m n p
+requires map_invariant v m n p ** pure (v =!= 0ul)
+ensures
+  OR.on_range (predicate_at m) 0 n **
+  pure (all_perms m 0 n 0.5R)
+{
+  rewrite (map_invariant v m n p)
+       as (OR.on_range (predicate_at m) 0 n ** pure (all_perms m 0 n 0.5R));
+}
+```
+
 let comp (c0:carrier) (c1:carrier { PM.composable_maps (PF.pcm_frac #small_vprop) c0 c1 })
 : carrier 
 = PM.compose_maps (PF.pcm_frac #small_vprop) c0 c1
@@ -125,13 +178,10 @@ requires emp
 ensures map_invariant 0ul (singleton 0 #0.5R p) 1 p
 {
   on_range_singleton p; //inlining the calc does not work
-  rewrite pure (p == OR.on_range (predicate_at (singleton 0 #0.5R p)) 0 1 /\ all_perms (singleton 0 #0.5R p) 0 1 0.5R)
-     as  map_invariant 0ul (singleton 0 #0.5R p) 1 p;
+  fold_map_invariant0 (singleton 0 #0.5R p) 1 p;
 }
 ```
 
-
-#push-options "--print_implicits"
 ```pulse
 fn new_barrier (p:storable)
 requires emp
@@ -166,17 +216,8 @@ ensures send b p ** recv b p
 }
 ```
 
-let unfold_map_invariant_0  (v:U32.t) (p:storable) (m:carrier) (n:nat)
-: Lemma
-  (requires v == 0ul)
-  (ensures map_invariant v m n p == pure (p == OR.on_range (predicate_at m) 0 n /\ all_perms m 0 n 0.5R))
-= ()
 
 module T = FStar.Tactics
-let apply_map_invariant_0_tac () = 
-  T.mapply (`vprop_equiv_ext);
-  // T.mapply (`unfold_map_invariant_0)
-  T.tadmit()
 
 ```pulse
 ghost
@@ -184,7 +225,6 @@ fn flip_map_invariant (v:U32.t) (p:storable) (m:carrier) (n:nat)
 requires map_invariant v m n p ** p ** pure (v == 0ul)
 ensures map_invariant 1ul m n p
 {
-  unfold_map_invariant_0 v p m n;
   rewrite each v as 0ul;
   rewrite (map_invariant 0ul m n p) as (map_invariant0 m n p);
   unfold map_invariant0;
@@ -216,7 +256,6 @@ ensures emp
   drop_ (inv b.i _)
 }
 ```
-#pop-options
 
 let composable (c0:carrier) (c1:carrier)
 = PM.composable_maps (PF.pcm_frac #small_vprop) c0 c1
@@ -288,12 +327,6 @@ let elim_predicate_at (m:carrier) (i:nat)
            up2 (fst (Some?.v (Map.sel m i)))) // ** pure (snd (Some?.v (Map.sel m i)) == 0.5R))
 = ()
 
-let apply_equiv (_:unit) : T.Tac unit = 
-  T.dump "A";
-  T.mapply (`vprop_equiv_ext);
-  T.dump "B";
-  T.tadmit()
-  // T.mapply (`elim_predicate_at)
 
 ```pulse
 ghost
@@ -493,13 +526,24 @@ let split_aux_post (b:barrier_t) (q r:storable)
     big_ghost_pcm_pts_to b.core.gref (singleton j #0.5R q) **
     big_ghost_pcm_pts_to b.core.gref (singleton k #0.5R r)
 
+
+
 ```pulse
 ghost
 fn map_invariant_all_perms v m n p
 requires map_invariant v m n p
 ensures  map_invariant v m n p ** pure (all_perms m 0 n 0.5R)
 {
-  admit()
+  if (v = 0ul)
+  {
+     unfold_map_invariant0 _ _ _ _;
+     fold_map_invariant0 m n p;
+     rewrite each 0ul as v;
+  }
+  else {
+    unfold_map_invariant1 _ _ _ _;
+    fold_map_invariant1 v m n p;
+  }
 }
 ```
 
@@ -516,7 +560,10 @@ ensures
   big_ghost_pcm_pts_to gref m **
   big_ghost_pcm_pts_to gref (empty_map_below n) **
   map_invariant v m n p **
-  pure (Map.sel m i == Some (down2 q, 0.5R) /\ i < n /\ all_perms m 0 n 0.5R)
+  pure (Map.sel m i == Some (down2 q, 0.5R) /\
+        i < n /\
+        all_perms m 0 n 0.5R /\
+        (forall j. n <= j ==> Map.sel m j == None))
 {
   map_invariant_all_perms v m n p;
   composable_three _ _ _ _;
@@ -566,22 +613,98 @@ ensures  GR.pts_to b.ctr (n + 1) **
          big_ghost_pcm_pts_to b.gref (singleton n #0.5R q) **
          big_ghost_pcm_pts_to b.gref (singleton n #0.5R q)
 {
-  admit()
+  GR.write b.ctr (n + 1);
+  down2_emp();
+  assert pure (Map.equal (empty_map_below n) (comp (singleton n #1.0R emp) (empty_map_below (n + 1))));
+  rewrite (big_ghost_pcm_pts_to b.gref (empty_map_below n))
+  as      (big_ghost_pcm_pts_to b.gref (comp (singleton n #1.0R emp) (empty_map_below (n + 1))));
+  big_ghost_share b.gref (singleton n #1.0R emp) (empty_map_below (n + 1));
+  big_ghost_write b.gref _ _
+   (PM.lift_frame_preserving_upd
+        _ _
+        (PF.mk_frame_preserving_upd (down2 emp) (down2 q))
+        (singleton n #1.0R emp)
+        n);
+  with m. assert (big_ghost_pcm_pts_to b.gref m);
+  assert pure (Map.equal m
+                         (comp (singleton n #0.5R q) (singleton n #0.5R q)));
+  rewrite (big_ghost_pcm_pts_to b.gref m)
+  as      (big_ghost_pcm_pts_to b.gref (comp (singleton n #0.5R q) (singleton n #0.5R q)));
+  big_ghost_share b.gref (singleton n #0.5R q) (singleton n #0.5R q);
 }
 ```
 
 let up_i (m:carrier) (i:nat) (p:storable) = Map.upd m i (Some (down2 p, 0.5R))
 let split_map (m:carrier) (i n:nat) (q r:storable) = (up_i (up_i (up_i m i emp) n q) (n + 1) r)
-```pulse
-ghost
-fn split_lemma (b:barrier_t_core) (m:carrier) (q r:storable) (i n:nat)
-requires pure (Map.sel m i == Some (down2 (q ** r), 0.5R))
-ensures pure (OR.on_range (predicate_at m) 0 n ==
-              OR.on_range (predicate_at (split_map m i n q r)) 0 (n + 2))
-{
-  admit()
-}
-```
+
+assume
+val on_range_eq_get (p:nat -> vprop) (i j k:nat)
+: Lemma 
+  (requires i <= j /\ j < k)
+  (ensures OR.on_range p i k == (OR.on_range p i j ** p j ** OR.on_range p (j + 1) k))
+
+assume
+val on_range_eq_snoc (p:nat -> vprop) (i j:nat)
+: Lemma 
+  (ensures OR.on_range p i (j + 1) == OR.on_range p i j ** p j)
+
+assume
+val on_range_frame (p q:nat -> vprop) (i j:nat)
+: Lemma 
+  (requires forall k. i <= k /\ k < j ==> p k == q k)
+  (ensures OR.on_range p i j == OR.on_range q i j)
+
+let star_assoc (p q r:vprop)
+: Lemma (p ** (q ** r) == (p ** q) ** r)
+= elim_vprop_equiv (vprop_equiv_assoc p q r)
+let star_comm (p q:vprop)
+: Lemma (p ** q == q ** p)
+= elim_vprop_equiv (vprop_equiv_comm p q)
+let emp_unit (p:vprop)
+: Lemma (emp ** p == p)
+= elim_vprop_equiv (vprop_equiv_unit p)
+
+let split_lemma (b:barrier_t_core) (m:carrier) (q r:storable) (i n:nat)
+: Lemma
+(requires i < n /\ Map.sel m i == Some (down2 (q ** r), 0.5R))
+(ensures OR.on_range (predicate_at m) 0 n ==
+         OR.on_range (predicate_at (split_map m i n q r)) 0 (n + 2))
+= let m' = (split_map m i n q r) in
+  calc (==) {
+    OR.on_range (predicate_at m) 0 n;
+  (==) { on_range_eq_get (predicate_at m) 0 i n }
+    OR.on_range (predicate_at m) 0 i **
+    up2 (down2 (q ** r)) **
+    OR.on_range (predicate_at m) (i + 1) n;
+  (==) { down2_star q r; up2_star (down2 q) (down2 r) }
+    OR.on_range (predicate_at m) 0 i **
+    (q ** r) **
+    OR.on_range (predicate_at m) (i + 1) n;
+  (==) { 
+         FStar.Classical.(
+          forall_intro_3 star_assoc;
+          forall_intro_2 star_comm;
+          forall_intro emp_unit 
+         )
+       }
+   (OR.on_range (predicate_at m) 0 i **
+    emp **
+    OR.on_range (predicate_at m) (i + 1) n) **
+    q ** r;
+  (==){
+        on_range_frame (predicate_at m) (predicate_at m') 0 i;
+        on_range_frame (predicate_at m) (predicate_at m') (i + 1) n
+      }
+    (OR.on_range (predicate_at m') 0 i **
+    emp ** 
+    OR.on_range (predicate_at m') (i + 1) n) ** q ** r;
+  (==) { on_range_eq_get (predicate_at m') 0 i n }
+    (OR.on_range (predicate_at m') 0 n ** q) ** r;
+  (==) { on_range_eq_snoc (predicate_at m') 0 n }
+    OR.on_range (predicate_at m') 0 (n + 1) ** r;
+  (==) { on_range_eq_snoc (predicate_at m') 0 (n + 1) }
+    OR.on_range (predicate_at m') 0 (n + 2);
+  }
 
 ```pulse
 ghost
@@ -598,8 +721,8 @@ ensures  barrier_inv b.core p ** split_aux_post b q r
   alloc r;
   big_ghost_gather b.core.gref m' (singleton n #0.5R q);
   big_ghost_gather b.core.gref (comp m' (singleton n #0.5R q)) (singleton (n + 1) #0.5R r);
-  assume_ (pure (Map.equal (comp (comp m' (singleton n #0.5R q)) (singleton (n + 1) #0.5R r))
-                           (split_map m i n q r)));
+  assert (pure (Map.equal (comp (comp m' (singleton n #0.5R q)) (singleton (n + 1) #0.5R r))
+                          (split_map m i n q r)));
   rewrite (big_ghost_pcm_pts_to b.core.gref (comp (comp m' (singleton n #0.5R q)) (singleton (n + 1) #0.5R r)))
        as (big_ghost_pcm_pts_to b.core.gref (split_map m i n q r));
   fold (split_aux_post b q r);
@@ -615,13 +738,10 @@ ensures  barrier_inv b.core p ** split_aux_post b q r
   }
   else
   {
-    rewrite (map_invariant v m n p) as (
-        OR.on_range (predicate_at (split_map m i n q r)) 0 (n + 2) **
-        pure (all_perms m 0 n 0.5R)
-    );
-    rewrite (OR.on_range (predicate_at (split_map m i n q r)) 0 (n + 2) **
-             pure (all_perms (split_map m i n q r) 0 (n + 2) 0.5R))
-        as (map_invariant v (split_map m i n q r) (n + 2) p);
+    unfold_map_invariant1 _ _ _ _;
+    rewrite (OR.on_range (predicate_at m) 0 n)
+    as      (OR.on_range (predicate_at (split_map m i n q r)) 0 (n + 2));
+    fold_map_invariant1 v (split_map m i n q r) (n + 2) p;
     fold_barrier_inv b.core p v (n + 2) (split_map m i n q r);
   }
  
@@ -647,268 +767,12 @@ opens (add_inv emp_inames b.i)
             big_ghost_pcm_pts_to b.core.gref (singleton k #0.5R r))
   {
     split_aux b p q r i;
+    unfold split_aux_post;
   };
   dup_inv _ _;
   fold (barrier b p);
   fold (recv b q);
   fold (barrier b p);
   fold (recv b r)
-}
-```
-
-
-let small_star = cm_small_vprop.mult
-let small_emp : small_vprop = cm_small_vprop.unit
-let small_emp_unit (x:small_vprop)
-: Lemma (small_star small_emp x == x)
-        [SMTPat (small_star small_emp x == x)]
-= cm_small_vprop.identity x
-let small_star_assoc (x y z:small_vprop)
-: Lemma (small_star x (small_star y z) == small_star (small_star x y) z)
-= cm_small_vprop.associativity x y z
-let small_star_comm (x y:small_vprop)
-: Lemma (small_star x y == small_star y x)
-        [SMTPat (small_star x y)]
-= cm_small_vprop.commutativity x y
-
-let up2_small_emp : squash (up2 small_emp == emp) = up2_emp()
-
-let down2_star (p q:storable)
-: Lemma (down2 (p ** q) == down2 p `small_star` down2 q)
-= down2_star p q
-
-let small_star_inj (p q r0 r1:small_vprop)
-: Lemma 
-  (p == q `small_star` r0 /\
-   p == q `small_star` r1 ==> r0 == r1)
-= admit() //!! not true !!!
-
-let up2_is_small (p:small_vprop)
-  : Lemma (is_small (up2 p))
-          [SMTPat (up2 p)]
-  = up2_is_small p
-
-let up2_small_star (p q:small_vprop)
-: Lemma (up2 (p `small_star` q) == (up2 p ** up2 q))
-= up2_star p q
-
-noeq
-type barrier_t_core = {
-  r: Box.box U32.t;
-  gref: core_ghost_pcm_ref;
-}
-
-noeq type barrier_t = {
-  core: barrier_t_core;
-  i: iref
-}
-
-let pcm_of (p:storable) = M.pcm_of cm_small_vprop (down2 p)
-
-let barrier_inv (b: barrier_t_core) (p:storable)
-: w:vprop { is_big w }
-= exists* v r q.
-    Box.pts_to b.r #0.5R v **
-    big_ghost_pcm_pts_to #_ #(pcm_of p) b.gref q **
-    up2 r **
-    pure(
-     if v = 0ul
-     then q == small_emp /\ r == small_emp
-     else down2 p == small_star q r
-    )
-
-let barrier (b: barrier_t) (p:storable)
-: vprop
-= inv b.i (barrier_inv b.core p)
-
-let send (b: barrier_t) (p:storable)
-: vprop
-= barrier b p **
-  Box.pts_to b.core.r #0.5R 0ul
-
-let recv (b:barrier_t) (q:storable)
-: vprop
-= exists* p.
-    barrier b p **
-    big_ghost_pcm_pts_to #_ #(pcm_of p) b.core.gref (down2 q)
-
-
-```pulse
-fn new_barrier (p:storable)
-requires emp
-returns b:barrier_t
-ensures send b p ** recv b p
-{
-  let r = Box.alloc 0ul;
-  let gref = big_ghost_alloc #_ #(pcm_of p) (down2 p);
-  let b = { r = r; gref = gref };
-  rewrite each r as b.r, gref as b.gref;
-  small_emp_unit (down2 p);
-  big_ghost_share #_ #(pcm_of p) b.gref small_emp (down2 p);
-  Box.share b.r;
-  rewrite emp as (up2 small_emp);
-  fold (barrier_inv b p);
-  let i = new_invariant (barrier_inv b p);
-  dup_inv _ _;
-  let bb = { core = b; i = i };
-  rewrite each b as bb.core;
-  rewrite each i as bb.i;
-  fold (barrier bb p);
-  fold (send bb p);
-  fold (barrier bb p);
-  fold (recv bb p);
-  bb
-}
-```
-
-```pulse
-fn signal (b:barrier_t) (#p:storable)
-requires send b p ** p
-ensures emp
-{
-  unfold send;
-  unfold barrier;
-  with_invariants b.i 
-  returns u:unit
-  ensures inv b.i (barrier_inv b.core p) ** emp
-  {
-    unfold barrier_inv;
-    Box.gather b.core.r;
-    with r. rewrite (up2 r) as emp;
-    with q. assert (big_ghost_pcm_pts_to #_ #(pcm_of p) b.core.gref q);
-    assert pure (q == small_emp);
-    write_atomic_box b.core.r 1ul;
-    Box.share b.core.r;
-    drop_ (Box.pts_to b.core.r #0.5R 1ul);
-    rewrite p as (up2 (down2 p));
-    small_emp_unit (down2 p);
-    assert pure (down2 p == small_star q (down2 p));
-    fold (barrier_inv b.core p);
-  };
-  drop_ (inv b.i _)
-}
-```
-
-let pcm_refine (#p:storable) (x:small_vprop)
-  : Lemma ((pcm_of p).refine x ==> x == down2 p)
-  = ()
-
-let extract_frame 
-      (p:storable) (claim:storable) (q:small_vprop)
-      (_:squash (FStar.PCM.compatible (pcm_of p) (small_star (down2 claim) q) (down2 p)))
-: Tot 
-  (frame:small_vprop {
-    q `small_star` (frame `small_star` down2 claim) == down2 p /\
-    (down2 claim `small_star` q) `small_star` frame == down2 p
-  })
-= let open FStar.PCM in
-  let frame = FStar.IndefiniteDescription.indefinite_description_tot _
-    (fun frame -> 
-      composable (pcm_of p)
-                 (small_star (down2 claim) q) frame /\
-      small_star frame (small_star (down2 claim) q) == (down2 p)) in
-  FStar.Classical.forall_intro_3 small_star_assoc;
-  frame
-
-```pulse
-fn rec wait_alt (b:barrier_t) (p claim:storable)
-requires barrier b p **
-         big_ghost_pcm_pts_to #_ #(pcm_of p) b.core.gref (down2 claim)
-ensures claim
-{
-  unfold barrier;
-  let res : bool =
-    with_invariants b.i
-    returns res:bool
-    ensures inv b.i (barrier_inv b.core p) **
-            (cond res claim (big_ghost_pcm_pts_to #_ #(pcm_of p) b.core.gref (down2 claim)))
-    {
-      unfold barrier_inv;
-      let v = read_atomic_box b.core.r;
-      if (v = 0ul)
-      {
-        intro_cond_false
-          claim
-          (big_ghost_pcm_pts_to #_ #(pcm_of p) b.core.gref (down2 claim));
-        fold (barrier_inv b.core p);
-        false;
-      }
-      else 
-      {
-        with r. assert (up2 r);
-        big_ghost_gather #_ #(pcm_of p) b.core.gref _ _;
-        with q. assert (big_ghost_pcm_pts_to #_ #(pcm_of p) b.core.gref (small_star (down2 claim) q));
-        assert pure (down2 p == small_star r q);
-        let x = big_ghost_read_simple #_ #(pcm_of p) b.core.gref;
-        pcm_refine #p x;
-        assert pure (x == down2 p);
-        assert pure (FStar.PCM.compatible (pcm_of p) (small_star (down2 claim) q) (down2 p));
-        let frame = extract_frame p claim q ();
-        //p == q ** r
-        //p == q ** (frame ** claim)
-        small_star_inj (down2 p) q (small_star frame (down2 claim)) r;
-        rewrite (up2 r) as (up2 (small_star frame (down2 claim)));
-        up2_small_star frame (down2 claim);
-        rewrite (up2 (small_star frame (down2 claim))) as
-                (up2 frame ** claim);
-        intro_cond_true
-            claim
-            (big_ghost_pcm_pts_to #_ #(pcm_of p) b.core.gref (down2 claim));
-        fold (barrier_inv b.core p);
-        true
-      }
-    };
-  if res
-  {
-    elim_cond_true _ _ _;
-    drop_ (inv b.i _);
-  }
-  else 
-  {
-    elim_cond_false _ _ _;
-    fold (barrier b p);
-    wait_alt b p claim;
-  }
-}
-```
-
-```pulse
-fn wait (b:barrier_t) (claim:storable)
-requires recv b claim
-ensures claim
-{
-  unfold recv;
-  wait_alt b _ claim
-}
-```
-
-```pulse
-ghost
-fn dup_barrier (b:barrier_t) (#p:storable)
-requires barrier b p
-ensures barrier b p ** barrier b p
-{
-  unfold barrier;
-  dup_inv _ _;
-  fold (barrier b p);
-  fold (barrier b p);
-}
-```
-
-```pulse
-ghost
-fn split (b:barrier_t) (#q r s:storable)
-requires recv b q ** pure (q == r ** s)
-ensures recv b r ** recv b s
-{
-  unfold recv;
-  with p. assert (barrier b p);
-  rewrite each q as (r ** s);
-  down2_star r s;
-  rewrite each (down2 (r ** s)) as (down2 r `small_star` down2 s);
-  big_ghost_share #_ #(pcm_of p) b.core.gref (down2 r) (down2 s);
-  dup_barrier b;
-  fold (recv b r);
-  fold (recv b s)
 }
 ```
